interpreter extraction

theories/interpreter_ppi.v
@@ -1,7 +1,7 @@
 From Wasm Require Import common properties tactic typing_inversion.
 From Coq Require Import ZArith.BinInt Program.Equality.
 From mathcomp Require Import ssreflect ssrfun ssrnat ssrbool eqtype seq.
-From Wasm Require Export operations host.
+From Wasm Require Export operations host type_preservation type_progress.
 Require Import BinNat.
 
 Set Implicit Arguments.
@@ -43,3 +43,59 @@ Definition config_tuple := config_tuple host_function.
 Definition host_state := host_state host_instance.
 
 End EmptyHost.
+
+
+Module Interpreter_PPI_extract.
+
+Import EmptyHost.
+
+Let t_progress := @t_progress host_function_eqType host_instance.
+
+Let t_preservation := @t_preservation host_function_eqType host_instance.
+
+Let config_typing := @config_typing host_function_eqType.
+
+
+Inductive res_ppi : Type :=
+| RSP_exhaustion
+| RSP_cfg: forall (hs: host_state) s f es ts,
+    config_typing s f es ts ->
+    res_ppi
+| RSP_terminal: forall es,
+    terminal_form es ->
+    res_ppi
+.
+
+Definition run_one_step_ppi (cfg: res_ppi): res_ppi.
+Proof.
+  destruct cfg as [| hs s f es ts Htype | Hterm].
+  - exact RSP_exhaustion.
+  - destruct (t_progress hs Htype) as [Hterm | [s' [f' [es' [hs' Hred]]]]].
+    + exact (RSP_cfg hs Htype).
+    + specialize (t_preservation Hred Htype) as Htype'.
+      by eapply RSP_cfg; eauto.
+  - by eapply RSP_terminal; eauto.
+Defined.
+
+Print run_one_step_ppi.
+
+Definition make_ppi_cfg s f es ts (Htype: config_typing s f es ts) : res_ppi :=
+  RSP_cfg tt Htype.
+
+(* This obviously terminate, but the only purpose of it is using the efficient N for extraction (instead of inserting extra proofs), so let's omit the proof *)
+Unset Guard Checking.
+
+Fixpoint run_multi_step_ppi (fuel: N) (cfg: res_ppi) {struct fuel}: res_ppi :=
+  match fuel with
+  | 0%N => RSP_exhaustion
+  | Npos p =>
+      match cfg with
+      | RSP_cfg hs s f es ts Htype =>
+          run_multi_step_ppi (Pos.pred_N p) (run_one_step_ppi (RSP_cfg hs Htype))
+      | x => x
+      end
+  end.
+
+Set Guard Checking.
+
+End Interpreter_PPI_extract.
